\documentclass{article}
\begin{document}

\begin{eqnarray*}
  \mbox{tf}(\mbox{\small term}_i, \mbox{\small doc}_m) = & \frac{| \{ w \in \mbox{\small doc}_m : w = \mbox{\small term}_i \} |} {| \{ w \in \mbox{\small doc}_m \} |} \\
  \mbox{idf}(\mbox{\small doc}_m) = & \frac{|D|}{| \{ d \in D : \mbox{\small term}_i \in \mbox{\small doc}_m \} | } \\
  \mbox{tf-idf}(\mbox{\small term}_i, \mbox{\small doc}_m) = & \mbox{\small tf}(\mbox{\small term}_i, \mbox{\small doc}_m) \times \mbox{\small idf}(\mbox{\small doc}_m)
\end{eqnarray*}
\end{document}